ToMathlib.lean
@@ -60,6 +60,8 @@ import ToMathlib.PFunctor.Cofree
 import ToMathlib.PFunctor.Equiv.Basic
 import ToMathlib.PFunctor.Free.Basic
 import ToMathlib.PFunctor.Free.Displayed
+import ToMathlib.PFunctor.Free.Displayed.Append
+import ToMathlib.PFunctor.Free.Displayed.Decoration
 import ToMathlib.PFunctor.Free.Path
 import ToMathlib.PFunctor.Lens.Basic
 import ToMathlib.PFunctor.Lens.Cartesian
